\documentclass[a4paper,12pt]{article}
\usepackage{amsmath}
\usepackage{enumitem}
\usepackage{geometry}
\usepackage{esvect}
\usepackage{textcomp}
\usepackage{siunitx}
\usepackage{microtype}
\usepackage{parskip}

\begin{document}
   \null\hfill\begin{tabular}[t]{l@{}}
      \textbf{Nama: Aldzikri Dwijayanto P.} \\
      \textbf{NIM:\@ 195410189} \\
      \textbf{Kelas: TI-4}
   \end{tabular} 

   \begin{enumerate}
      \item Diketahui vector $\underline{u} = (3, 2, -1) ; \underline{v} = (2, 6, 7) $; dan $\underline{w} = (0, 2, 3)$ Hitung 
      \begin{enumerate}[label=\alph*.]
         \item $\underline{u} \cdot \underline{v}$
         \item $\underline{u} - \underline{v}$
         \item $3(7\underline{u} -\underline{v})$
         \item $\underline{u} \times (\underline{v} \times \underline{w})$ \\[4ex]
      \end{enumerate}

      Jawab
      \begin{enumerate}[label= (\alph*)]
         \item 
         $
         \begin{aligned}
            \underline{u} \cdot \underline{v} 
            &= (3)(2) + (2)(6) + (-1)(7) \\
            &= 6 + 12 + (-7) \\
            &= 11
         \end{aligned}
         $\\[2ex]

         \item
         $
         \begin{aligned}
            \underline{u} - \underline{v}
            &= (3 - 2 , 2 - 6 , -1 -7) \\
            &= (1, -4, -8)
         \end{aligned}
         $\\[2ex]

         \item 
         $
         \begin{aligned}
            3(7\underline{u} - \underline{v})
            &= 21\underline{u} - 3\underline{v} \\
            &= (63 - 6 , 42 - 18 , -21 - 21) \\
            &= (57, 24, -42)
         \end{aligned}
         $\\[2ex]

         \item
         $
         \begin{aligned}
             \underline{u} \times (\underline{v} \times \underline{w})
             &= (\underline{u} \cdot \underline{w})\underline{v} - (\underline{u} \cdot \underline{v})\underline{w} \\
             &= (1)\underline{v} - 11\underline{w} \\
             &= (2, 6, 7) - (0, 22, 33) \\
             &= (2, -16, -26)
         \end{aligned}
         $\\[4ex]
      \end{enumerate}

      \item 
      Diketahui $u = (2, -1, 1) ; v = (1, 1, 2)$\\
      Hitung
      \begin{enumerate}[label=\alph*.]
        \item $u + 2v$
        \item $||u|| , ||v||$
        \item Sudut antara \textit{u} dan \textit{v}\\[4ex]
      \end{enumerate}


      Jawab
      \begin{enumerate}[label=(\alph*)]
        \item
        $
        \begin{aligned}
           u + 2v
           &= (2 + 2, -1 + 2, 1 + 4) \\
           &= (4, 1, 5)
        \end{aligned}
        $\\[2ex]

        \item 
        $
        \begin{aligned}
           ||u||
           &= \sqrt{(2^{2} + (-1)^{2} + 1^{2})} \\
           &= \sqrt{4 + 1 + 1} \\
           &= \sqrt{6}
        \end{aligned}
        $\\[2ex]

        $
        \begin{aligned}
           ||v||
           &= \sqrt{1^{2} + 1^{2} + 2^{2}} \\
           &= \sqrt{6}
        \end{aligned}
        $\\[2ex]

        \item Sudut antara $u$ dan $v$\\
        $u \cdot v = 3$ \\
        $||u|| = \sqrt{6}$ \\
        $||v|| = \sqrt{6}$ \\
        $
        \begin{aligned}
           \cos \theta
           &= \frac{\vv{u} \cdot \vv{v}}{|\vv{u}| |\vv{v}|} \\
           &= \frac{3}{\sqrt{6} \sqrt{6}} \\
           &= \frac{3}{6} \\
           &= \frac{1}{2} \\
           &= \ang{60} 
        \end{aligned}
        $\\[4ex]
      \end{enumerate}

      \item Tentukan jarak antara $P_{1}$ dan $P_{2}$ jika $P_{1}$ $(0, -1, -6)$ ; $P_{2}$ $(2, -4, 8)$! \\
      Jawab \\
          $
          \begin{aligned}
             d
             &= \sqrt{(x_{2} - x_{1})^{2} + (y_{2} - y_{1})^{2} + (2_{2} - 2_{1})^{2}} \\
             &= \sqrt{4 + 9 + 196} \\
             &= \sqrt{209}
          \end{aligned}
          $\\[4ex]

     \item Selesaikan SPL berikut \\
     $-3x + 4y + 6z = 30$ \\
     $-x - 2y + 3z = 8$ \\
     $x + z = 6$\\[4ex]

     Jawab \\
     $-3x + 4y + 6z = 30$ \\
     $-x - 2y + 3z = 8$ \\
     $x + z = 6$
     $\\
     \rightarrow \begin{bmatrix}
        -3 & 4 & 6 \\
        -1 & -2 & 3 \\
        1 & 0 & 1
     \end{bmatrix}
     \quad
     \begin{bmatrix}
        x \\
        y \\
        z \\
     \end{bmatrix}
     =\begin{bmatrix}
        36 \\
        8 \\
        6
     \end{bmatrix}
     $

     $
     \begin{bmatrix}
        x \\
        y \\
        z
     \end{bmatrix}
     =\begin{bmatrix}
        -3 & 4 & 6 \\
        -1 & -2 & 3 \\
        1 & 0 & 1
     \end{bmatrix}^{-1}
     \quad
     \begin{bmatrix}
        30 \\
        8 \\
        6
     \end{bmatrix}
     $

     $
     =\frac{1}{34}\begin{bmatrix}
        -2 & -4 & 24 \\
        -4 & -9 & 3 \\
        2 & 4 & 10
     \end{bmatrix}
     \quad
     \begin{bmatrix}
        30 \\
        8 \\
        6
     \end{bmatrix}
     $

     $
     =\begin{bmatrix}
        \frac{-1}{17} & \frac{-2}{17} & \frac{12}{17} \\[6pt] 
        \frac{2}{17} & \frac{-9}{34} & \frac{3}{34} \\[6pt] 
        \frac{1}{17} & \frac{2}{17} & \frac{5}{17}
     \end{bmatrix}
     \quad
     \begin{bmatrix}
        30 \\
        8 \\
        6
     \end{bmatrix}
     $

     $
     =\begin{bmatrix}
        \frac{26}{17} \\[6pt]
        \frac{33}{17} \\[6pt]
        \frac{76}{17}
     \end{bmatrix}
     $
   \end{enumerate}
\end{document}
